\def\VCDate{2018/03/04}\def\VCVersion{74613b4}
\documentclass{ffslides}
\ffpage{42}{\numexpr 16/9}
\usepackage{ProofPower,amsmath}
\begin{document}
\obeyspaces

\normalpage{CS113 LAB 3 - Example 3.3}{
Example 3.3\\
Show that $\sim (p \rightarrow q) \equiv p \land (\sim q)$\\
\input ex3
\begin{align}
 \sim (p \rightarrow q) & \equiv \sim (\sim p \lor q)          \tag{Conditional} \\
                        & \equiv \sim (\sim p) \land (\sim q)  \tag{De Morgan's} \\
                        & \equiv p \land (\sim q) \, \PrLA{}         \tag{Double Negation} 
\end{align}
\begin{GFT}{SML}
\+val L0 = asm\_rule \PrKM{} \PrLD{}(p \PrLE{} q) \PrKO{};\\
\+val T = \PrKM{} \PrLD{}(p \PrLE{} q) \PrKE{} \PrLD{}(\PrLD{}p \PrLC{} q) \PrKO{};\\
\+val conditional = prove\_rule [ ] T;\\
\+val L1 = rewrite\_rule [conditional] L0;\\
\+rewrite\_rule [\PrLD{}\_\PrLC{}\_thm] L1;\\
\end{GFT}
}
\btext{.05}{.32}{.35}{Notice that ProofPower automatically applied the double-negation rule}
\putfig{.05}{.65}{.50}{ex3}

\normalpage{CS113 LAB 3 - Example 3.5}{
Example 3.5\\
Show that $p \rightarrow q \equiv \sim q \rightarrow \sim p$ \\
\input ex5
\begin{align}
 p \rightarrow q & \equiv (\sim p) \lor q		 \tag{Conditional}\\
		 & \equiv \sim [p \land (\sim q)]	 \tag{De Morgan's}\\
		 & \equiv \sim [(\sim q) \land p]	 \tag{Commutative}\\
		 & \equiv [\sim (\sim q)] \lor (\sim p)  \tag{De Morgan's}\\
		 & \equiv q \lor (\sim p)		 \tag{Double Negation}\\
		 & \equiv \sim q \rightarrow \sim p \, \PrLA{} \tag{Conditional}
\end{align}
\begin{GFT}{SML}
\+val L0 = asm\_rule \PrKM{} p \PrLE{} q \PrKO{};\\
\+val L1 = rewrite\_rule [\PrLE{}\_thm] L0;\\
\+val T = \PrKM{} \PrLD{}p \PrLC{} q \PrKE{} \PrLD{}(p \PrLB{} \PrLD{}q) \PrKO{};\\
\+val demorgan = prove\_rule [ ] T;\\
\+val L2 = rewrite\_rule [demorgan] L1;\\
\+val T = \PrKM{} p \PrLB{} \PrLD{}q \PrKE{} \PrLD{}q \PrLB{} p \PrKO{};\\
\+val commutative = prove\_rule [ ] T;\\
\+val L3 = rewrite\_rule [commutative] L2;\\
\+val L4 = rewrite\_rule [\PrLD{}\_\PrLB{}\_thm] L3;\\
\+val T = \PrKM{} q \PrLC{} \PrLD{}p \PrKE{} \PrLD{}q \PrLE{} \PrLD{}p \PrKO{};\\
\+val conditional = prove\_rule [ ] T;\\
\+rewrite\_rule [conditional] L4;\\
\end{GFT}
}
\btext{.05}{.32}{.35}{Notice that ProofPower automatically applied conditional rule and double-negation rule}
\putfig{.30}{.60}{.35}{ex5}

\normalpage{CS113 LAB 3 - Problem 3.8}{
Problem 3.8\\
Show that $\sim (p \leftrightarrow q) \equiv (p \land \sim q) \lor (\sim p \land q)$\\
\input{p8}
\begin{align}
 \sim (p \leftrightarrow q) & \equiv \sim[(p \rightarrow q) \land (q \rightarrow p)]
			      \tag{Biconditional}\\
			    & \equiv [\sim(p \rightarrow q)] \lor [\sim (q \rightarrow p)]
			      \tag{De Morgan's}\\
			    & \equiv (p \land \sim q) \lor (\sim p \land q) \, \PrLA{}
			      \tag{Conditional}
\end{align}
\begin{GFT}{SML}
\+val L0 = asm\_rule \PrKM{} \PrLD{}(p \PrKE{} q) \PrKO{};\\
\+val L1 = rewrite\_rule [\PrKE{}\_thm] L0;\\
\+val T = \PrKM{} \PrLD{}((p \PrLE{} q) \PrLB{} (q \PrLE{} p)) \PrKE{} (\PrLD{}(p \PrLE{} q)) \PrLC{} (\PrLD{}(q \PrLE{} p)) \PrKO{};\\
\+val demorgan = prove\_rule [ ] T;\\
\+val L2 = rewrite\_rule [demorgan] L1;\\
\+rewrite\_rule [\PrLD{}\_\PrLE{}\_thm] L2;\\
\end{GFT}
}
\btext{.05}{.32}{.35}{Notice that ProofPower automatically applied biconditional rule}
\putfig{.05}{.65}{.50}{p8}

\normalpage{CS113 LAB 3 - Problem 3.11}{
Problem 3.11\\
Show using a chain of logical equivalences that $(p \rightarrow r) \land (q \rightarrow r) \equiv (p \lor q) \rightarrow r$\\
\input{p11}
\begin{align}
(p \land q) \rightarrow r & \equiv [\sim (p \lor q)] \lor r						   \tag{Conditional}\\
			  & \equiv [(\sim p) \land (\sim q)] \lor r 					   \tag{De Morgan's}\\
			  & \equiv [\sim p \lor r] \land [(\sim q)] \lor r				   \tag{Distributive}\\
			  & \equiv (p \rightarrow r) \land (q \rightarrow r) \, \PrLA{}			   \tag{Conditional}
\end{align}
\begin{GFT}{SML}
\+val L0 = asm\_rule \PrKM{} \PrLD{}(p \PrKE{} q) \PrKO{};\\
\+val L1 = rewrite\_rule [\PrKE{}\_thm] L0;\\
\+val T = \PrKM{} \PrLD{}((p \PrLE{} q) \PrLB{} (q \PrLE{} p)) \PrKE{} (\PrLD{}(p \PrLE{} q)) \PrLC{} (\PrLD{}(q \PrLE{} p)) \PrKO{};\\
\+val demorgan = prove\_rule [ ] T;\\
\+val L2 = rewrite\_rule [demorgan] L1; \\
\+val L3 = rewrite\_rule [\PrLD{}\_\PrLE{}\_thm] L2;\\
\end{GFT}
}
\btext{.05}{.45}{.35}{Notice that ProofPower automatically applied biconditional rule and conditional rule}
\putfig{.05}{.77}{.40}{p11}

\normalpage{CS113 LAB 3 - Problem 3.12}{
Problem 3.12\\
Show using a chain of logical equivalences that $p \leftrightarrow q \equiv (p \land q) \lor (\sim p \land \sim q)$\\
\input{p12}
\begin{align}
p \leftrightarrow q & \equiv (p \rightarrow q) \land (q \rightarrow p)
		      \tag{Biconditional}\\
		    & \equiv (\sim p \lor q) \land (\sim q \lor p)
		      \tag{Conditional}\\
		    & \equiv [\sim p \land (\sim q \lor p)] \lor [q \land (\sim q \lor p)]
		      \tag{Distributive OR}\\
		    & \equiv [(\sim p \land \sim q) \lor (\sim p \land p)] \lor [(q \land \sim 				     q) \lor (q \land p)]
		      \tag{Distributive AND}\\
		    & \equiv [(\sim p \land \sim q) \lor c] \lor [c \lor (q \land p)]
		      \tag{Contradiction}\\
		    & \equiv (\sim p \land \sim q) \lor (p \land q)
		      \tag{Identity}\\
		    & \equiv (p \land q) \lor (\sim p \land \sim q) \, \PrLA{}
		      \tag{Commutative}
\end{align}
}
\btext{.05}{.32}{.30}{Notice that ProofPower automatically applied biconditional rule and conditional rule}

\normalpage{CS113 LAB 3 - Problem 3.12}{
\begin{GFT}{SML}
\+val L0 = asm\_rule \PrKM{} (p \PrKE{} q) \PrKO{};\\
\+val L1 = rewrite\_rule [\PrKE{}\_thm] L0;\\
\+val L2 = rewrite\_rule [\PrLE{}\_thm] L1;\\
\+val T = \PrKM{} (\PrLD{}p \PrLC{} q) \PrLB{} (\PrLD{}q \PrLC{} p) \PrKE{} (\PrLD{}p \PrLB{} (\PrLD{}q \PrLC{} p)) \PrLC{} (q \PrLB{} (\PrLD{}q \PrLC{} p)) \PrKO{};\\
\+val distributiveOR = prove\_rule [ ] T;\\
\+val L3 = rewrite\_rule [distributiveOR] L2;\\
\+val T = \PrKM{} (\PrLD{}p \PrLB{} (\PrLD{}q \PrLC{} p)) \PrLC{} (q \PrLB{} (\PrLD{}q \PrLC{} p)) \PrKE{} ((\PrLD{}p \PrLB{} \PrLD{}q) \PrLC{} (\PrLD{}p \PrLB{} p)) \PrLC{} ((q \PrLB{} \PrLD{}q) \PrLC{} (q \PrLB{} p)) \PrKO{};\\
\+val distributiveAND = prove\_rule [ ] T;\\
\+val L4 = rewrite\_rule [distributiveAND] L3;\\
\+val T = \PrKM{} ((\PrLD{}p \PrLB{} \PrLD{}q) \PrLC{} (\PrLD{}p \PrLB{} p)) \PrLC{} ((q \PrLB{} \PrLD{}q) \PrLC{} (q \PrLB{} p)) \PrKE{} ((\PrLD{}p \PrLB{} \PrLD{}q) \PrLC{} F) \PrLC{} (F \PrLC{} (q \PrLB{} p)) \PrKO{};\\
\+val contradiction = prove\_rule [ ] T;\\
\+val L5 = rewrite\_rule [contradiction] L4;\\
\+val T = \PrKM{} (\PrLD{}p \PrLB{} \PrLD{}q) \PrLC{} (q \PrLB{} p) \PrKE{} (p \PrLB{} q) \PrLC{} (\PrLD{}p \PrLB{} \PrLD{}q) \PrKO{};\\
\+val commutative = prove\_rule [ ] T;\\
\+val L6 = rewrite\_rule [commutative] L5;\\
\end{GFT}
}

\normalpage{CS113 LAB 3 - Problem 3.12}{}
\putfig{.05}{.15}{.70}{p12}

\end{document}

